ironfleet/src/Dafny/Distributed/Protocol/ZooKeeper/PerformamceProof/EmptyDiffInvariants.dfy
@@ -1,0 +1,43 @@
+include "../../../Impl/Common/SeqIsUniqueDef.i.dfy"
+include "../../../Common/Framework/EnvironmentTCP.s.dfy"
+include "../Timestamps/TimestampedType.dfy"
+include "TimestampedLS.dfy"
+
+include "../Types.dfy"
+include "../DistributedSystem.dfy"
+include "../ZKEnvironment.dfy"
+include "../ZKDatabase.dfy"
+include "../Follower.dfy"
+include "../Leader.dfy"
+include "../LearnerHandler.dfy"
+include "Definitions.dfy"
+
+
+/* This module contains invariants that have nothing to do with performance */
+module Zookeeper_EmptyDiffInvariants {
+import opened Common__SeqIsUniqueDef_i
+import opened ZKTimestamp
+import opened ZooKeeper_Types
+import opened ZooKeeper_Environment
+import opened ZooKeeper_DistributedSystem
+import opened EnvironmentTCP_s
+import opened ZooKeeper_ZKDatabase
+import opened ZooKeeper_Follower
+import opened ZooKeeper_Leader
+import opened ZooKeeper_LearnerHandler
+import opened Zookeeper_Performance_Definitions
+import opened ZooKeeper_TimestampedDistributedSystem
+
+
+/*****************************************************************************************
+*                                    Empty Diff facts                                    *
+*****************************************************************************************/
+
+predicate EmptyDiff_Invariant(tls:TLS_State) {
+    forall pkt | pkt in tls.t_environment.sentPackets ::
+        && !pkt.msg.v.SyncSNAP?
+        && !pkt.msg.v.SyncTRUNC?
+        && !pkt.msg.v.Commit?
+}
+
+}
